proof/invariant-abstract/ARM/ArchCrunchSetup_AI.thy
@@ -15,6 +15,7 @@ imports
 begin
 context ARM begin
 
+
 crunch_ignore (add: debugPrint invalidateTLB_ASID invalidateTLB_VAASID cleanByVA
   cleanByVA_PoU invalidateByVA invalidateByVA_I invalidate_I_PoU
   cleanInvalByVA branchFlush clean_D_PoU cleanInvalidate_D_PoC cleanInvalidateL2Range
