proof/invariant-abstract/ARM/ArchKHeap_AI.thy
@@ -1,0 +1,101 @@
+(*
+ * Copyright 2014, General Dynamics C4 Systems
+ *
+ * This software may be distributed and modified according to the terms of
+ * the GNU General Public License version 2. Note that NO WARRANTY is provided.
+ * See "LICENSE_GPLv2.txt" for details.
+ *
+ * @TAG(GD_GPL)
+ *)
+
+theory ArchKHeap_AI
+imports "../KHeapPre_AI"
+begin
+
+context ARM begin
+
+
+lemma pspace_in_kernel_window_atyp_lift_strong:
+  assumes atyp_inv: "\<And>P p T. \<lbrace>\<lambda>s. P (typ_at T p s)\<rbrace> f \<lbrace>\<lambda>rv s. P (typ_at T p s)\<rbrace>"
+  assumes arch_inv: "\<And>P. \<lbrace>\<lambda>s. P (arm_kernel_vspace (arch_state s))\<rbrace> f \<lbrace>\<lambda>r s. P (arm_kernel_vspace (arch_state s))\<rbrace>"
+  shows      "\<lbrace>\<lambda>s. pspace_in_kernel_window s\<rbrace> f \<lbrace>\<lambda>rv s. pspace_in_kernel_window s\<rbrace>"
+  apply (simp add: pspace_in_kernel_window_def)
+  apply (rule hoare_lift_Pf[where f="\<lambda>s. arm_kernel_vspace (arch_state s)", OF _ arch_inv])
+   apply (rule hoare_vcg_all_lift)
+   apply (simp add: obj_bits_T)
+   apply (simp add: valid_def)
+  apply clarsimp
+  subgoal for _ x s _ _ ko
+  apply (cases "kheap s x")
+  apply (frule use_valid[OF _ atyp_inv, where P1= "\<lambda>x. \<not> x" and T1="a_type ko" and p1=x];
+          simp add: obj_at_def a_type_def)
+
+   subgoal for ko'
+   apply (drule spec[of _ ko'])
+   apply (simp add: obj_bits_T)
+   apply (frule use_valid[OF _ atyp_inv, where P1= "\<lambda>x. x" and T1="a_type ko'" and p1=x])
+   by (simp add: obj_at_def a_type_def)+
+ done
+ done
+
+lemma pspace_in_kernel_window_atyp_lift:
+  assumes atyp_inv: "\<And>P p T. \<lbrace>\<lambda>s. P (typ_at T p s)\<rbrace> f \<lbrace>\<lambda>rv s. P (typ_at T p s)\<rbrace>"
+  assumes arch_inv: "\<And>P. \<lbrace>\<lambda>s. P (arch_state s)\<rbrace> f \<lbrace>\<lambda>r s. P (arch_state s)\<rbrace>"
+  shows      "\<lbrace>\<lambda>s. pspace_in_kernel_window s\<rbrace> f \<lbrace>\<lambda>rv s. pspace_in_kernel_window s\<rbrace>"
+  by (rule pspace_in_kernel_window_atyp_lift_strong[OF atyp_inv arch_inv])
+
+
+lemma cap_refs_in_kernel_window_arch_update[simp]:
+  "arm_kernel_vspace (f (arch_state s)) = arm_kernel_vspace (arch_state s)
+     \<Longrightarrow> cap_refs_in_kernel_window (arch_state_update f s) = cap_refs_in_kernel_window s"
+  by (simp add: cap_refs_in_kernel_window_def not_kernel_window_arch_def)
+
+
+lemma
+  ex_ako_at_def2: 
+  "(\<exists>ko. ako_at ko p s \<and> P ko) = (aobj_at P p s)"
+  by (simp add: aobj_at_def)
+
+lemma vs_lookup_aobj_at_lift:
+  assumes obj_at: "\<And>P P' p. \<lbrace>\<lambda>s. P (aobj_at P' p s)\<rbrace> f \<lbrace>\<lambda>r s. P (aobj_at P' p s)\<rbrace>"
+  assumes arch_state: "\<And>P. \<lbrace>\<lambda>s. P (arch_state s)\<rbrace> f \<lbrace>\<lambda>r s. P (arch_state s)\<rbrace>"
+  shows "\<lbrace>\<lambda>s. P (vs_lookup s)\<rbrace> f \<lbrace>\<lambda>rv s. P (vs_lookup s)\<rbrace>"
+  apply (simp add: vs_lookup_def vs_lookup1_def)
+  apply (simp add: ex_ako_at_def2)
+  apply (rule hoare_lift_Pf[where f="arch_state", OF _ arch_state])
+  apply (rule hoare_lift_Pf[where f="\<lambda>s rs p rs' p'. aobj_at (P' p rs rs' p') p s" for P'])
+   apply (rule hoare_vcg_prop)
+  apply (clarsimp simp add: valid_def)
+  apply (erule_tac P=P in rsubst)
+  apply (rule ext)+
+  apply (erule use_valid, rule obj_at, simp)
+  done
+
+lemma vs_lookup_pages_aobj_at_lift:
+  assumes obj_at: "\<And>P P' p. \<lbrace>\<lambda>s. P (aobj_at P' p s)\<rbrace> f \<lbrace>\<lambda>r s. P (aobj_at P' p s)\<rbrace>"
+  assumes arch_state: "\<And>P. \<lbrace>\<lambda>s. P (arch_state s)\<rbrace> f \<lbrace>\<lambda>r s. P (arch_state s)\<rbrace>"
+  shows "\<lbrace>\<lambda>s. P (vs_lookup_pages s)\<rbrace> f \<lbrace>\<lambda>rv s. P (vs_lookup_pages s)\<rbrace>"
+  apply (simp add: vs_lookup_pages_def vs_lookup_pages1_def)
+  apply (simp add: ex_ako_at_def2)
+  apply (rule hoare_lift_Pf[where f="arch_state", OF _ arch_state])
+  apply (rule hoare_lift_Pf[where f="\<lambda>s rs p rs' p'. aobj_at (P' p rs rs' p') p s" for P'])
+   apply (rule hoare_vcg_prop)
+  apply (clarsimp simp add: valid_def)
+  apply (erule_tac P=P in rsubst)
+  apply (rule ext)+
+  apply (erule use_valid, rule obj_at, simp)
+  done
+
+lemma valid_arch_objs_lift_weak:
+  assumes obj_at: "\<And>P P' p. \<lbrace>\<lambda>s. P (aobj_at P' p s)\<rbrace> f \<lbrace>\<lambda>r s. P (aobj_at P' p s)\<rbrace>"
+  assumes arch_state: "\<And>P. \<lbrace>\<lambda>s. P (arch_state s)\<rbrace> f \<lbrace>\<lambda>r s. P (arch_state s)\<rbrace>"
+  shows "\<lbrace>valid_arch_objs\<rbrace> f \<lbrace>\<lambda>_. valid_arch_objs\<rbrace>"
+  apply (rule valid_arch_objs_lift)
+    apply (rule vs_lookup_aobj_at_lift)
+     apply (rule obj_at arch_state)+
+  done
+
+end
+  
+
+end
