proof/invariant-abstract/KHeapPre_AI.thy
@@ -1,0 +1,45 @@
+(*
+ * Copyright 2014, General Dynamics C4 Systems
+ *
+ * This software may be distributed and modified according to the terms of
+ * the GNU General Public License version 2. Note that NO WARRANTY is provided.
+ * See "LICENSE_GPLv2.txt" for details.
+ *
+ * @TAG(GD_GPL)
+ *)
+
+theory KHeapPre_AI
+imports "./$L4V_ARCH/Machine_AI"
+begin
+
+primrec
+  same_caps :: "Structures_A.kernel_object \<Rightarrow> Structures_A.kernel_object \<Rightarrow> bool"
+where
+  "same_caps val (CNode sz cs)       = (val = CNode sz cs)"
+| "same_caps val (TCB tcb)           = (\<exists>tcb'. val = TCB tcb'
+                                         \<and> (\<forall>(getF, t) \<in> ran tcb_cap_cases. getF tcb' = getF tcb))"
+| "same_caps val (Endpoint ep)       = is_ep val"
+| "same_caps val (Notification ntfn) = is_ntfn val"
+| "same_caps val (ArchObj ao)        = (\<exists>ao'. val = ArchObj ao')"
+
+
+lemma same_caps_more_simps[simp]:
+ "same_caps (CNode sz cs) val       = (val = CNode sz cs)"
+ "same_caps (TCB tcb)     val       = (\<exists>tcb'. val = TCB tcb'
+                                         \<and> (\<forall>(getF, t) \<in> ran tcb_cap_cases. getF tcb' = getF tcb))"
+ "same_caps (Endpoint ep) val       = is_ep val"
+ "same_caps (Notification ntfn) val = is_ntfn val"
+ "same_caps (ArchObj ao) val        = (\<exists>ao'. val = ArchObj ao')"
+ by (cases val, (fastforce simp: is_obj_defs)+)+
+
+lemma dmo_return [simp]:
+  "do_machine_op (return x) = return x"
+  by (simp add: do_machine_op_def select_f_def return_def gets_def get_def 
+                bind_def modify_def put_def)
+
+fun
+  non_arch_obj :: "kernel_object \<Rightarrow> bool" where
+  "non_arch_obj (ArchObj _) = False"
+  | "non_arch_obj _ = True"
+
+end
